Foundation/IntProp/Kripke/DP.lean
@@ -8,10 +8,9 @@ open Formula Formula.Kripke
 
 namespace Kripke
 
-variable {α}
-variable {φ ψ : Formula α}
+variable {φ ψ : Formula ℕ}
 
-abbrev IntDPCounterexampleFrame (F₁ : Kripke.Frame) (F₂ : Kripke.Frame) (w₁ : F₁.World) (w₂ : F₂.World) : Kripke.Frame where
+abbrev counterexampleDPFrame (F₁ : Kripke.Frame) (F₂ : Kripke.Frame) (w₁ : F₁.World) (w₂ : F₂.World) : Kripke.Frame where
   World := Unit ⊕ F₁.World ⊕ F₂.World;
   Rel x y :=
     match x, y with
@@ -21,127 +20,101 @@ abbrev IntDPCounterexampleFrame (F₁ : Kripke.Frame) (F₂ : Kripke.Frame) (w�
     | (Sum.inr $ Sum.inl x), (Sum.inr $ Sum.inl y) => F₁.Rel x y
     | (Sum.inr $ Sum.inr x), (Sum.inr $ Sum.inr y) => F₂.Rel x y
     | _, _ => False
+  rel_po := {
+    refl := by simp only [Sum.forall, implies_true, Frame.rel_refl, and_self];
+    trans := by
+      simp only [Sum.forall, true_implies, imp_self, implies_true, true_and, false_implies, and_true, and_self, forall_const, imp_false];
+      constructor;
+      . constructor;
+        . intro _ _; apply F₁.rel_trans;
+        . intro _ _; apply F₂.rel_trans;
+      . constructor;
+        . intro _ _ _; apply F₁.rel_trans;
+        . intro _ _ _; apply F₂.rel_trans;
+    antisymm := by
+      simp only [Sum.forall, imp_self, implies_true, reduceCtorEq, and_self, imp_false, false_implies, Sum.inr.injEq, true_and, Sum.inl.injEq, and_true];
+      constructor;
+      . intro _ _; apply F₁.rel_antisymm;
+      . intro _ _; apply F₂.rel_antisymm;
+  }
 
-lemma IntDPCounterexampleFrame.reflexive
-  {F₁ : Kripke.Frame} {F₂ : Kripke.Frame}
-  {w₁ : F₁.World} {w₂ : F₂.World}
-  (F₁_refl : Reflexive F₁.Rel) (F₂_refl : Reflexive F₂.Rel)
-  : Reflexive (IntDPCounterexampleFrame F₁ F₂ w₁ w₂).Rel := by
-  simp only [Reflexive, Sum.forall, forall_const, true_and];
-  constructor;
-  . exact F₁_refl;
-  . exact F₂_refl;
+abbrev counterexampleDPModel (M₁ : Kripke.Model) (M₂ : Kripke.Model) (w₁ : M₁.World) (w₂ : M₂.World) : Model where
+  toFrame := counterexampleDPFrame M₁.toFrame M₂.toFrame w₁ w₂;
+  Val := ⟨
+    λ w a =>
+      match w with
+      | Sum.inr $ Sum.inl w => M₁ w a
+      | Sum.inr $ Sum.inr w => M₂ w a
+      | _ => False,
+    by
+      simp only [Sum.forall, imp_false, not_false_eq_true, implies_true, imp_self, false_implies, and_self, and_true, true_and];
+      constructor;
+      . intro _ _; apply M₁.Val.hereditary;
+      . intro _ _; apply M₂.Val.hereditary;
+  ⟩
 
-lemma IntDPCounterexampleFrame.transitive
-  {F₁ : Kripke.Frame} {F₂ : Kripke.Frame}
-  {w₁ : F₁.World} {w₂ : F₂.World}
-  (F₁_trans : Transitive F₁.Rel) (F₂_trans : Transitive F₂.Rel)
-  : Transitive (IntDPCounterexampleFrame F₁ F₂ w₁ w₂).Rel := by
-  simp only [Transitive, Sum.forall, forall_true_left, imp_self, forall_const, true_and, IsEmpty.forall_iff, implies_true, and_true, and_self, imp_false];
-  constructor;
-  . constructor;
-    . intro _ _; apply F₁_trans;
-    . intro _ _; apply F₂_trans;
-  . constructor;
-    . intro _ _; apply F₁_trans;
-    . intro _ _; apply F₂_trans;
+variable {M₁ : Kripke.Model} {M₂ : Kripke.Model}
 
-lemma IntDPCounterexampleFrame.antisymmetric
-  {F₁ : Kripke.Frame} {F₂ : Kripke.Frame}
-  {w₁ : F₁.World} {w₂ : F₂.World}
-  (F₁_antisymm : Antisymmetric F₁.Rel) (F₂_antisymm : Antisymmetric F₂.Rel)
-  : Antisymmetric (IntDPCounterexampleFrame F₁ F₂ w₁ w₂).Rel := by
-  simp only [Antisymmetric, Sum.forall, forall_true_left, forall_const, IsEmpty.forall_iff, implies_true, and_self, imp_false, Sum.inr.injEq, true_and, Sum.inl.injEq, and_true];
-  constructor;
-  . exact F₁_antisymm;
-  . exact F₂_antisymm;
-
-abbrev IntDPCounterexampleModel (M₁ : Kripke.Model α) (M₂ : Kripke.Model α) (w₁ : M₁.World) (w₂ : M₂.World) : Kripke.Model α where
-  Frame := IntDPCounterexampleFrame M₁.Frame M₂.Frame w₁ w₂;
-  Valuation w a :=
-    match w with
-    | Sum.inr $ Sum.inl w => M₁.Valuation w a
-    | Sum.inr $ Sum.inr w => M₂.Valuation w a
-    | _ => False
-
-lemma IntDPCounterexampleModel.atomic_hereditary
-  {M₁ : Kripke.Model α} {M₂ : Kripke.Model α}
-  {w₁ : M₁.World} {w₂ : M₂.World}
-  (M₁_hered : M₁.Valuation.atomic_hereditary) (M₂_hered : M₂.Valuation.atomic_hereditary)
-  : (IntDPCounterexampleModel M₁ M₂ w₁ w₂).Valuation.atomic_hereditary := by
-  simp;
-  constructor;
-  . apply M₁_hered;
-  . apply M₂_hered;
-
-variable {M₁ : Kripke.Model α} {M₂ : Kripke.Model α}
-
-lemma satisfies_left_on_IntDPCounterexampleModel :
-  (Satisfies M₁ w φ) ↔ (Satisfies (IntDPCounterexampleModel M₁ M₂ w₁ w₂) (Sum.inr $ Sum.inl w) φ) := by
+lemma satisfies_left_on_counterexampleDPModel :
+  w ⊧ φ ↔ (Satisfies (counterexampleDPModel M₁ M₂ w₁ w₂) (Sum.inr $ Sum.inl w) φ) := by
   induction φ using rec' generalizing w with
   | himp φ ψ ihp ihq =>
     constructor;
     . intro hpq X hWX hp;
-      obtain ⟨x, hx, ex⟩ : ∃ x, (M₁.Frame.Rel w x) ∧ (Sum.inr $ Sum.inl x) = X := by
-        replace hWX : (IntDPCounterexampleModel M₁ M₂ w₁ w₂).Frame.Rel _ X := hWX;
-        simp [IntDPCounterexampleFrame] at hWX;
+      obtain ⟨x, hx, ex⟩ : ∃ x, (M₁.Rel w x) ∧ (Sum.inr $ Sum.inl x) = X := by
+        replace hWX : (counterexampleDPModel M₁ M₂ w₁ w₂).Rel _ X := hWX;
+        simp [counterexampleDPModel] at hWX;
         split at hWX;
         all_goals simp_all;
       subst ex;
       exact ihq.mp $ hpq hx $ ihp.mpr hp;
     . intro h v Rwv hp;
       apply @ihq v |>.mpr $ h (by simpa) $ ihp.mp hp;
-  | _ => simp_all [IntDPCounterexampleModel, Satisfies.iff_models, Satisfies];
+  | _ => simp_all [counterexampleDPModel, Satisfies.iff_models, Satisfies];
 
-lemma satisfies_right_on_IntDPCounterexampleModel :
-  (Satisfies M₂ w φ) ↔ (Satisfies (IntDPCounterexampleModel M₁ M₂ w₁ w₂) (Sum.inr $ Sum.inr w) φ) := by
+lemma satisfies_right_on_counterexampleDPModel :
+  w ⊧ φ ↔ (Satisfies (counterexampleDPModel M₁ M₂ w₁ w₂) (Sum.inr $ Sum.inr w) φ) := by
   induction φ using rec' generalizing w with
   | himp φ ψ ihp ihq =>
     constructor;
     . intro h X hWX hp;
-      obtain ⟨x, hx, ex⟩ : ∃ x, (M₂.Frame.Rel w x) ∧ (Sum.inr $ Sum.inr x) = X := by
-        replace hWX : (IntDPCounterexampleModel M₁ M₂ w₁ w₂).Frame.Rel _ X := hWX;
-        simp [IntDPCounterexampleFrame] at hWX;
+      obtain ⟨x, hx, ex⟩ : ∃ x, (M₂.Rel w x) ∧ (Sum.inr $ Sum.inr x) = X := by
+        replace hWX : (counterexampleDPModel M₁ M₂ w₁ w₂).Rel _ X := hWX;
+        simp [counterexampleDPModel] at hWX;
         split at hWX;
         all_goals simp_all;
       subst ex;
       exact ihq.mp $ h hx $ ihp.mpr hp;
     . intro h v Rwv hp;
       exact ihq.mpr $ h (by simpa) $ ihp.mp hp;
-  | _ => simp_all [IntDPCounterexampleModel, Satisfies.iff_models, Satisfies];
-
-theorem disjunctive_int [Inhabited α] [DecidableEq α] [Encodable α] : (Hilbert.Int α) ⊢! φ ⋎ ψ → (Hilbert.Int α) ⊢! φ ∨ (Hilbert.Int α) ⊢! ψ := by
-  contrapose;
-  intro hC; push_neg at hC;
-  have ⟨hnp, hnq⟩ := hC;
-  obtain ⟨Fp, Fp_refl, Fp_trans, Vp, Vp_hered, wp, hp⟩ := by simpa [Semantics.Realize, ValidOnFrame, ValidOnModel] using not_imp_not.mpr Int_complete.complete hnp;
-  obtain ⟨Fq, Fq_refl, Fq_trans, Vq, Vq_hered, wq, hq⟩ := by simpa [Semantics.Realize, ValidOnFrame, ValidOnModel] using not_imp_not.mpr Int_complete.complete hnq;
-  apply (not_imp_not.mpr Int_sound.sound);
-  simp [Semantics.Realize, ValidOnFrame, ValidOnModel, Satisfies];
-  use (IntDPCounterexampleFrame Fp Fq wp wq);
-  refine ⟨IntDPCounterexampleFrame.reflexive Fp_refl Fq_refl, IntDPCounterexampleFrame.transitive Fp_trans Fq_trans, ?_⟩;
-  use (IntDPCounterexampleModel ⟨Fp, Vp⟩ ⟨Fq, Vq⟩ wp wq).Valuation;
-  constructor;
-  . exact IntDPCounterexampleModel.atomic_hereditary (M₁ := ⟨Fp, Vp⟩) (M₂ := ⟨Fq, Vq⟩) Vp_hered Vq_hered;
-  . use (Sum.inl ());
-    constructor;
-    . exact not_imp_not.mpr
-        (Satisfies.formula_hereditary
-          (M := IntDPCounterexampleModel ⟨Fp, Vp⟩ ⟨Fq, Vq⟩ wp wq)
-          (IntDPCounterexampleModel.atomic_hereditary Vp_hered Vq_hered)
-          (IntDPCounterexampleFrame.transitive Fp_trans Fq_trans)
-          (w := Sum.inl ()) (w' := Sum.inr $ Sum.inl wp) (by aesop))
-        $ satisfies_left_on_IntDPCounterexampleModel |>.not.mp hp;
-    . exact not_imp_not.mpr
-        (Satisfies.formula_hereditary
-          (M := IntDPCounterexampleModel ⟨Fp, Vp⟩ ⟨Fq, Vq⟩ wp wq)
-          (IntDPCounterexampleModel.atomic_hereditary Vp_hered Vq_hered)
-          (IntDPCounterexampleFrame.transitive Fp_trans Fq_trans)
-          (w := Sum.inl ()) (w' := Sum.inr $ Sum.inr wq) (by aesop))
-        $ satisfies_right_on_IntDPCounterexampleModel |>.not.mp hq;
-
-instance [DecidableEq α] [Inhabited α] [Encodable α] : Disjunctive (Hilbert.Int α) := ⟨disjunctive_int⟩
+  | _ => simp_all [counterexampleDPModel, Satisfies.iff_models, Satisfies];
 
 end Kripke
+
+namespace Hilbert.Int
+
+theorem disjunctive : (Hilbert.Int ℕ) ⊢! φ ⋎ ψ → (Hilbert.Int ℕ) ⊢! φ ∨ (Hilbert.Int ℕ) ⊢! ψ := by
+  contrapose;
+  intro hC; push_neg at hC;
+  have ⟨hnφ, hnψ⟩ := hC;
+  obtain ⟨F₁, V₁, w₁, hφ⟩ := by simpa [ValidOnFrame, ValidOnModel] using not_imp_not.mpr Int.Kripke.complete.complete hnφ;
+  obtain ⟨F₂, V₂, w₂, hψ⟩ := by simpa [ValidOnFrame, ValidOnModel] using not_imp_not.mpr Int.Kripke.complete.complete hnψ;
+  apply (not_imp_not.mpr Int.Kripke.sound.sound);
+  simp [ValidOnFrame, ValidOnModel];
+  let M := Kripke.counterexampleDPModel ⟨F₁, V₁⟩ ⟨F₂, V₂⟩ w₁ w₂;
+  use M.toFrame, M.Val, (Sum.inl ());
+  apply Formula.Kripke.Satisfies.or_def.not.mpr;
+  push_neg;
+  constructor;
+  . have := not_imp_not.mpr $ @Satisfies.formula_hereditary (M := M) (w := Sum.inl ()) (w' := Sum.inr $ Sum.inl w₁) φ (by simp);
+    apply this;
+    exact Kripke.satisfies_left_on_counterexampleDPModel.not.mp hφ;
+  . have := not_imp_not.mpr $ @Satisfies.formula_hereditary (M := M) (w := Sum.inl ()) (w' := Sum.inr $ Sum.inr w₂) ψ (by simp);
+    apply this;
+    exact Kripke.satisfies_right_on_counterexampleDPModel.not.mp hψ;
+
+instance : Disjunctive (Hilbert.Int ℕ) := ⟨disjunctive⟩
+
+end Hilbert.Int
 
 end LO.IntProp
